csim (closed simulation) -> rsim (runtime simulation).

theories/lambda_lang/rsim/definition.v
@@ -1,7 +1,7 @@
 From simuliris Require Import
   prelude.
 From simuliris.lambda_lang Require Export
-  csim.bisubst.
+  rsim.bisubst.
 From simuliris.lambda_lang Require Import
   sim.notations.
 
@@ -11,14 +11,14 @@ Section sim_GS.
   Context (Χ : sim_protocol Σ).
   Implicit Types Γ : bisubst.
 
-  Definition csim Φ eₛ eₜ : iProp Σ :=
+  Definition rsim Φ eₛ eₜ : iProp Σ :=
     ∀ Γ eₛ' eₜ',
     ⌜eₛ' = eₛ.[Γ.ₛ#] ∧ eₜ' = eₜ.[Γ.ₜ#]⌝ -∗
     bisubst_well_formed Γ -∗
     SIM eₛ' ≳ eₜ' [[ Χ ]] {{ Φ }}.
-  #[global] Arguments csim _%I (_ _)%lambda_expr : assert.
+  #[global] Arguments rsim _%I (_ _)%lambda_expr : assert.
 
-  Definition csimv Φ eₛ eₜ : iProp Σ :=
-    csim (sim_post_vals Φ) eₛ eₜ.
-  #[global] Arguments csimv _%I (_ _)%lambda_expr : assert.
+  Definition rsimv Φ eₛ eₜ : iProp Σ :=
+    rsim (sim_post_vals Φ) eₛ eₜ.
+  #[global] Arguments rsimv _%I (_ _)%lambda_expr : assert.
 End sim_GS.
