theories/lambda_lang/rsim/rules.v
@@ -4,10 +4,10 @@ From simuliris.lambda_lang Require Export
   well_formed.
 From simuliris.lambda_lang Require Export
   sim.derived_rules
-  csim.definition.
+  rsim.definition.
 From simuliris.lambda_lang Require Import
   sim.proofmode
-  csim.notations.
+  rsim.notations.
 
 Section sim_GS.
   Context `{sim_programs : !SimPrograms lambda_ectx_lang lambda_ectx_lang}.
@@ -18,52 +18,52 @@ Section sim_GS.
   Implicit Types v vₛ vₜ : lambda_val.
   Implicit Types e eₛ eₜ : lambda_expr.
 
-  #[local] Ltac csim_intro :=
+  #[local] Ltac rsim_intro :=
     iIntros "%Γ % % (-> & ->) #HΓ"; sim_simpl.
 
-  Section csim.
+  Section rsim.
     Implicit Types Φ : lambda_expr → lambda_expr → iProp Σ.
 
-    Lemma csim_mono Φ1 Φ2 eₛ eₜ :
+    Lemma rsim_mono Φ1 Φ2 eₛ eₜ :
       (∀ eₛ eₜ, Φ1 eₛ eₜ -∗ Φ2 eₛ eₜ) -∗
       SIM eₛ ⩾ eₜ [[ Χ ]] {{ Φ1 }} -∗
       SIM eₛ ⩾ eₜ [[ Χ ]] {{ Φ2 }}.
     Proof.
-      iIntros "HΦ Hcsim". csim_intro.
-      sim_mono "Hcsim".
+      iIntros "HΦ Hrsim". rsim_intro.
+      sim_mono "Hrsim".
     Qed.
 
-    Lemma cupd_csim Φ eₛ eₜ :
+    Lemma cupd_rsim Φ eₛ eₜ :
       (|++> SIM eₛ ⩾ eₜ [[ Χ ]] {{ Φ }}) ⊢
       SIM eₛ ⩾ eₜ [[ Χ ]] {{ Φ }}.
     Proof.
-      iIntros "Hcsim". csim_intro.
-      iMod "Hcsim". iSmash.
+      iIntros "Hrsim". rsim_intro.
+      iMod "Hrsim". iSmash.
     Qed.
-    Lemma bupd_csim Φ eₛ eₜ :
+    Lemma bupd_rsim Φ eₛ eₜ :
       (|==> SIM eₛ ⩾ eₜ [[ Χ ]] {{ Φ }}) ⊢
       SIM eₛ ⩾ eₜ [[ Χ ]] {{ Φ }}.
     Proof.
-      iIntros "Hcsim". csim_intro.
-      iMod "Hcsim". iSmash.
+      iIntros "Hrsim". rsim_intro.
+      iMod "Hrsim". iSmash.
     Qed.
 
-    Lemma csim_cupd Φ eₛ eₜ :
+    Lemma rsim_cupd Φ eₛ eₜ :
       SIM eₛ ⩾ eₜ [[ Χ ]] {{ λ eₛ eₜ, |++> Φ eₛ eₜ }} ⊢
       SIM eₛ ⩾ eₜ [[ Χ ]] {{ Φ }}.
     Proof.
-      iIntros "Hcsim". csim_intro.
+      iIntros "Hrsim". rsim_intro.
       sim_cupd. iSmash.
     Qed.
-    Lemma csim_bupd Φ eₛ eₜ :
+    Lemma rsim_bupd Φ eₛ eₜ :
       SIM eₛ ⩾ eₜ [[ Χ ]] {{ λ eₛ eₜ, |==> Φ eₛ eₜ }} ⊢
       SIM eₛ ⩾ eₜ [[ Χ ]] {{ Φ }}.
     Proof.
-      iIntros "Hcsim". csim_intro.
+      iIntros "Hrsim". rsim_intro.
       sim_bupd. iSmash.
     Qed.
 
-    Lemma csim_val Φ v :
+    Lemma rsim_val Φ v :
       lambda_val_well_formed sim_progₛ v →
       ( ∀ vₛ vₜ,
         vₛ ≈ vₜ -∗
@@ -71,36 +71,36 @@ Section sim_GS.
       ) ⊢
       SIM v ⩾ v [[ Χ ]] {{ Φ }}.
     Proof.
-      iIntros "%Hwf HΦ". csim_intro.
+      iIntros "%Hwf HΦ". rsim_intro.
       sim_post. iApply "HΦ". lambda_expr_simplifier.
     Qed.
 
-    Lemma csim_var Φ x :
+    Lemma rsim_var Φ x :
       ( ∀ vₛ vₜ,
         vₛ ≈ vₜ -∗
         Φ vₛ vₜ
       ) ⊢
       SIM $x ⩾ $x [[ Χ ]] {{ Φ }}.
     Proof.
-      iIntros "HΦ". csim_intro.
+      iIntros "HΦ". rsim_intro.
       sim_post.
     Qed.
 
-    Lemma csim_let Φ eₛ1 eₛ2 eₜ1 eₜ2 :
+    Lemma rsim_let Φ eₛ1 eₛ2 eₜ1 eₜ2 :
       SIM eₜ1 ⩾ eₛ1 [[ Χ ]] {{# (≈) }} -∗
       SIM eₜ2 ⩾ eₛ2 [[ Χ ]] {{ Φ }} -∗
       SIM let: eₜ1 in eₜ2 ⩾ let: eₛ1 in eₛ2 [[ Χ ]] {{ Φ }}.
     Proof.
-      iIntros "Hcsim1 Hcsim2". csim_intro.
-      sim_apply (sim_let with "(Hcsim1 [//] HΓ)"). iIntros "%vₛ1 %vₜ1 #Hv1".
+      iIntros "Hrsim1 Hrsim2". rsim_intro.
+      sim_apply (sim_let with "(Hrsim1 [//] HΓ)"). iIntros "%vₛ1 %vₜ1 #Hv1".
       sim_asimpl.
       sim_evalₛ (rewrite (bisubst_consₛ _ vₜ1)).
       sim_evalₜ (rewrite (bisubst_consₜ vₛ1)).
-      sim_apply ("Hcsim2" with "[//]").
+      sim_apply ("Hrsim2" with "[//]").
       iApply bisubst_cons_well_formed; iSmash.
     Qed.
 
-    Lemma csim_call Φ eₛ1 eₛ2 eₜ1 eₜ2 :
+    Lemma rsim_call Φ eₛ1 eₛ2 eₜ1 eₜ2 :
       SIM eₜ1 ⩾ eₛ1 [[ Χ ]] {{# (≈) }} -∗
       SIM eₜ2 ⩾ eₛ2 [[ Χ ]] {{# (≈) }} -∗
       ( ∀ func vₛ vₜ,
@@ -110,11 +110,11 @@ Section sim_GS.
       ) -∗
       SIM eₜ1 eₜ2 ⩾ eₛ1 eₛ2 [[ Χ ]] {{ Φ }}.
     Proof.
-      iIntros "Hcsim1 Hcsim2 Hsim". csim_intro.
-      sim_apply (sim_call with "(Hcsim1 [//] HΓ) (Hcsim2 [//] HΓ) Hsim").
+      iIntros "Hrsim1 Hrsim2 Hsim". rsim_intro.
+      sim_apply (sim_call with "(Hrsim1 [//] HΓ) (Hrsim2 [//] HΓ) Hsim").
     Qed.
 
-    Lemma csim_unop Φ op eₛ eₜ :
+    Lemma rsim_unop Φ op eₛ eₜ :
       SIM eₛ ⩾ eₜ [[ Χ ]] {{# (≈) }} -∗
       ( ∀ vₛ vₜ,
         vₛ ≈ vₜ -∗
@@ -122,11 +122,11 @@ Section sim_GS.
       ) -∗
       SIM LambdaUnop op eₛ ⩾ LambdaUnop op eₜ [[ Χ ]] {{ Φ }}.
     Proof.
-      iIntros "Hcsim HΦ". csim_intro.
-      sim_apply (sim_unop with "(Hcsim [//] HΓ)").
+      iIntros "Hrsim HΦ". rsim_intro.
+      sim_apply (sim_unop with "(Hrsim [//] HΓ)").
     Qed.
 
-    Lemma csim_binop Φ op eₛ1 eₛ2 eₜ1 eₜ2 :
+    Lemma rsim_binop Φ op eₛ1 eₛ2 eₜ1 eₜ2 :
       SIM eₛ1 ⩾ eₜ1 [[ Χ ]] {{# (≈) }} -∗
       SIM eₛ2 ⩾ eₜ2 [[ Χ ]] {{# (≈) }} -∗
       ( ∀ vₛ vₜ,
@@ -135,25 +135,25 @@ Section sim_GS.
       ) -∗
       SIM LambdaBinop op eₛ1 eₛ2 ⩾ LambdaBinop op eₜ1 eₜ2 [[ Χ ]] {{ Φ }}.
     Proof.
-      iIntros "Hcsim1 Hcsim2 HΦ". csim_intro.
-      sim_apply (sim_binop with "(Hcsim1 [//] HΓ) (Hcsim2 [//] HΓ)").
+      iIntros "Hrsim1 Hrsim2 HΦ". rsim_intro.
+      sim_apply (sim_binop with "(Hrsim1 [//] HΓ) (Hrsim2 [//] HΓ)").
     Qed.
 
-    Lemma csim_if Φ eₛ0 eₛ1 eₛ2 eₜ0 eₜ1 eₜ2 :
+    Lemma rsim_if Φ eₛ0 eₛ1 eₛ2 eₜ0 eₜ1 eₜ2 :
       SIM eₛ0 ⩾ eₜ0 [[ Χ ]] {{# (≈) }} -∗
       ( SIM eₛ1 ⩾ eₜ1 [[ Χ ]] {{ Φ }} ∧
         SIM eₛ2 ⩾ eₜ2 [[ Χ ]] {{ Φ }}
       ) -∗
       SIM LambdaIf eₛ0 eₛ1 eₛ2 ⩾ LambdaIf eₜ0 eₜ1 eₜ2 [[ Χ ]] {{ Φ }}.
     Proof.
-      iIntros "Hcsim0 Hcsim12". csim_intro.
-      sim_apply (sim_if with "(Hcsim0 [//] HΓ)").
+      iIntros "Hrsim0 Hrsim12". rsim_intro.
+      sim_apply (sim_if with "(Hrsim0 [//] HΓ)").
       iSplit.
-      - iDestruct "Hcsim12" as "(Hcsim1 & _)". iSmash.
-      - iDestruct "Hcsim12" as "(_ & Hcsim2)". iSmash.
+      - iDestruct "Hrsim12" as "(Hrsim1 & _)". iSmash.
+      - iDestruct "Hrsim12" as "(_ & Hrsim2)". iSmash.
     Qed.
 
-    Lemma csim_constr Φ tag eₛ1 eₛ2 eₜ1 eₜ2 :
+    Lemma rsim_constr Φ tag eₛ1 eₛ2 eₜ1 eₜ2 :
       SIM eₛ1 ⩾ eₜ1 [[ Χ ]] {{# (≈) }} -∗
       SIM eₛ2 ⩾ eₜ2 [[ Χ ]] {{# (≈) }} -∗
       ( ∀ vₛ vₜ,
@@ -162,10 +162,10 @@ Section sim_GS.
       ) -∗
       SIM &tag eₛ1 eₛ2 ⩾ &tag eₜ1 eₜ2 [[ Χ ]] {{ Φ }}.
     Proof.
-      iIntros "Hcsim1 Hcsim2 HΦ". csim_intro.
-      sim_apply (sim_constr with "(Hcsim1 [//] HΓ) (Hcsim2 [//] HΓ)").
+      iIntros "Hrsim1 Hrsim2 HΦ". rsim_intro.
+      sim_apply (sim_constr with "(Hrsim1 [//] HΓ) (Hrsim2 [//] HΓ)").
     Qed.
-    Lemma csim_constr_valₜ1 Φ tag eₛ eₜ :
+    Lemma rsim_constr_valₜ1 Φ tag eₛ eₜ :
       SIM eₛ ⩾ eₜ [[ Χ ]] {{# (≈) }} -∗
       ( ∀ vₛ lₜ vₜ,
         (lₜ +ₗ 0) ↦ₜ tag -∗
@@ -176,10 +176,10 @@ Section sim_GS.
       ) -∗
       SIM eₛ ⩾ &tag eₜ #() [[ Χ ]] {{ Φ }}.
     Proof.
-      iIntros "Hcsim HΦ". csim_intro.
-      sim_apply (sim_constr_valₜ1 with "(Hcsim [//] HΓ)").
+      iIntros "Hrsim HΦ". rsim_intro.
+      sim_apply (sim_constr_valₜ1 with "(Hrsim [//] HΓ)").
     Qed.
-    Lemma csim_constr_valₜ2 Φ tag eₛ eₜ :
+    Lemma rsim_constr_valₜ2 Φ tag eₛ eₜ :
       SIM eₛ ⩾ eₜ [[ Χ ]] {{# (≈) }} -∗
       ( ∀ vₛ lₜ vₜ,
         (lₜ +ₗ 0) ↦ₜ tag -∗
@@ -190,11 +190,11 @@ Section sim_GS.
       ) -∗
       SIM eₛ ⩾ &tag #() eₜ [[ Χ ]] {{ Φ }}.
     Proof.
-      iIntros "Hcsim HΦ". csim_intro.
-      sim_apply (sim_constr_valₜ2 with "(Hcsim [//] HΓ)").
+      iIntros "Hrsim HΦ". rsim_intro.
+      sim_apply (sim_constr_valₜ2 with "(Hrsim [//] HΓ)").
     Qed.
 
-    Lemma csim_load Φ eₛ1 eₛ2 eₜ1 eₜ2 :
+    Lemma rsim_load Φ eₛ1 eₛ2 eₜ1 eₜ2 :
       SIM eₛ1 ⩾ eₜ1 [[ Χ ]] {{# (≈) }} -∗
       SIM eₛ2 ⩾ eₜ2 [[ Χ ]] {{# (≈) }} -∗
       ( ∀ vₛ vₜ,
@@ -203,50 +203,50 @@ Section sim_GS.
       ) -∗
       SIM ![eₛ2] eₛ1 ⩾ ![eₜ2] eₜ1 [[ Χ ]] {{ Φ }}.
     Proof.
-      iIntros "Hcsim1 Hcsim2 HΦ". csim_intro.
-      sim_apply (derived_rules.sim_load with "(Hcsim1 [//] HΓ) (Hcsim2 [//] HΓ)").
+      iIntros "Hrsim1 Hrsim2 HΦ". rsim_intro.
+      sim_apply (derived_rules.sim_load with "(Hrsim1 [//] HΓ) (Hrsim2 [//] HΓ)").
     Qed.
 
-    Lemma csim_store Φ eₛ1 eₛ2 eₛ3 eₜ1 eₜ2 eₜ3 :
+    Lemma rsim_store Φ eₛ1 eₛ2 eₛ3 eₜ1 eₜ2 eₜ3 :
       SIM eₛ1 ⩾ eₜ1 [[ Χ ]] {{# (≈) }} -∗
       SIM eₛ2 ⩾ eₜ2 [[ Χ ]] {{# (≈) }} -∗
       SIM eₛ3 ⩾ eₜ3 [[ Χ ]] {{# (≈) }} -∗
       Φ #() #() -∗
       SIM eₛ1 <-[eₛ2]- eₛ3 ⩾ eₜ1 <-[eₜ2]- eₜ3 [[ Χ ]] {{ Φ }}.
     Proof.
-      iIntros "Hcsim1 Hcsim2 Hcsim3 HΦ". csim_intro.
-      sim_apply (derived_rules.sim_store with "(Hcsim1 [//] HΓ) (Hcsim2 [//] HΓ) (Hcsim3 [//] HΓ)").
+      iIntros "Hrsim1 Hrsim2 Hrsim3 HΦ". rsim_intro.
+      sim_apply (derived_rules.sim_store with "(Hrsim1 [//] HΓ) (Hrsim2 [//] HΓ) (Hrsim3 [//] HΓ)").
     Qed.
-  End csim.
+  End rsim.
 
-  Section csimv.
+  Section rsimv.
     Implicit Types Φ : lambda_val → lambda_val → iProp Σ.
 
-    Lemma csimv_mono Φ1 Φ2 eₛ eₜ :
+    Lemma rsimv_mono Φ1 Φ2 eₛ eₜ :
       (∀ vₛ vₜ, Φ1 vₛ vₜ -∗ Φ2 vₛ vₜ) -∗
       SIM eₛ ⩾ eₜ [[ Χ ]] {{# Φ1 }} -∗
       SIM eₛ ⩾ eₜ [[ Χ ]] {{# Φ2 }}.
     Proof.
-      iIntros "HΦ Hcsim". csim_intro.
-      sim_mono "Hcsim".
+      iIntros "HΦ Hrsim". rsim_intro.
+      sim_mono "Hrsim".
     Qed.
 
-    Lemma csimv_cupd Φ eₛ eₜ :
+    Lemma rsimv_cupd Φ eₛ eₜ :
       SIM eₛ ⩾ eₜ [[ Χ ]] {{# λ vₛ vₜ, |++> Φ vₛ vₜ }} ⊢
       SIM eₛ ⩾ eₜ [[ Χ ]] {{# Φ }}.
     Proof.
-      iIntros "Hcsim". csim_intro.
+      iIntros "Hrsim". rsim_intro.
       sim_cupd. iSmash.
     Qed.
-    Lemma csimv_bupd Φ eₛ eₜ :
+    Lemma rsimv_bupd Φ eₛ eₜ :
       SIM eₛ ⩾ eₜ [[ Χ ]] {{# λ vₛ vₜ, |==> Φ vₛ vₜ }} ⊢
       SIM eₛ ⩾ eₜ [[ Χ ]] {{# Φ }}.
     Proof.
-      iIntros "Hcsim". csim_intro.
+      iIntros "Hrsim". rsim_intro.
       sim_bupd. iSmash.
     Qed.
 
-    Lemma csimv_val Φ v :
+    Lemma rsimv_val Φ v :
       lambda_val_well_formed sim_progₛ v →
       ( ∀ vₛ vₜ,
         vₛ ≈ vₜ -∗
@@ -255,11 +255,11 @@ Section sim_GS.
       SIM v ⩾ v [[ Χ ]] {{# Φ }}.
     Proof.
       iIntros "%Hwf HΦ".
-      iApply csim_val; first done.
+      iApply rsim_val; first done.
       rewrite sim_post_vals_unseal /sim_post_vals'. iSmash.
     Qed.
 
-    Lemma csimv_var Φ x :
+    Lemma rsimv_var Φ x :
       ( ∀ vₛ vₜ,
         vₛ ≈ vₜ -∗
         Φ vₛ vₜ
@@ -267,11 +267,11 @@ Section sim_GS.
       SIM $x ⩾ $x [[ Χ ]] {{# Φ }}.
     Proof.
       iIntros "HΦ".
-      iApply csim_var.
+      iApply rsim_var.
       rewrite sim_post_vals_unseal /sim_post_vals'. iSmash.
     Qed.
 
-    Lemma csimv_unop Φ op eₛ eₜ :
+    Lemma rsimv_unop Φ op eₛ eₜ :
       SIM eₛ ⩾ eₜ [[ Χ ]] {{# (≈) }} -∗
       ( ∀ vₛ vₜ,
         vₛ ≈ vₜ -∗
@@ -280,11 +280,11 @@ Section sim_GS.
       SIM LambdaUnop op eₛ ⩾ LambdaUnop op eₜ [[ Χ ]] {{# Φ }}.
     Proof.
       iIntros "Hsim HΦ".
-      iApply (csim_unop with "Hsim").
+      iApply (rsim_unop with "Hsim").
       rewrite sim_post_vals_unseal /sim_post_vals'. iSmash.
     Qed.
 
-    Lemma csimv_binop Φ op eₛ1 eₛ2 eₜ1 eₜ2 :
+    Lemma rsimv_binop Φ op eₛ1 eₛ2 eₜ1 eₜ2 :
       SIM eₛ1 ⩾ eₜ1 [[ Χ ]] {{# (≈) }} -∗
       SIM eₛ2 ⩾ eₜ2 [[ Χ ]] {{# (≈) }} -∗
       ( ∀ vₛ vₜ,
@@ -294,11 +294,11 @@ Section sim_GS.
       SIM LambdaBinop op eₛ1 eₛ2 ⩾ LambdaBinop op eₜ1 eₜ2 [[ Χ ]] {{# Φ }}.
     Proof.
       iIntros "Hsim1 Hsim2 HΦ".
-      iApply (csim_binop with "Hsim1 Hsim2").
+      iApply (rsim_binop with "Hsim1 Hsim2").
       rewrite sim_post_vals_unseal /sim_post_vals'. iSmash.
     Qed.
 
-    Lemma csimv_constr Φ tag eₛ1 eₛ2 eₜ1 eₜ2 :
+    Lemma rsimv_constr Φ tag eₛ1 eₛ2 eₜ1 eₜ2 :
       SIM eₛ1 ⩾ eₜ1 [[ Χ ]] {{# (≈) }} -∗
       SIM eₛ2 ⩾ eₜ2 [[ Χ ]] {{# (≈) }} -∗
       ( ∀ vₛ vₜ,
@@ -308,10 +308,10 @@ Section sim_GS.
       SIM &tag eₛ1 eₛ2 ⩾ &tag eₜ1 eₜ2 [[ Χ ]] {{# Φ }}.
     Proof.
       iIntros "Hsim1 Hsim2 HΦ".
-      iApply (csim_constr with "Hsim1 Hsim2").
+      iApply (rsim_constr with "Hsim1 Hsim2").
       rewrite sim_post_vals_unseal /sim_post_vals'. iSmash.
     Qed.
-    Lemma csimv_constr_valₜ1 Φ tag eₛ eₜ :
+    Lemma rsimv_constr_valₜ1 Φ tag eₛ eₜ :
       SIM eₛ ⩾ eₜ [[ Χ ]] {{# (≈) }} -∗
       ( ∀ vₛ lₜ vₜ,
         (lₜ +ₗ 0) ↦ₜ tag -∗
@@ -323,10 +323,10 @@ Section sim_GS.
       SIM eₛ ⩾ &tag eₜ #() [[ Χ ]] {{# Φ }}.
     Proof.
       iIntros "Hsim HΦ".
-      iApply (csim_constr_valₜ1 with "Hsim").
+      iApply (rsim_constr_valₜ1 with "Hsim").
       rewrite sim_post_vals_unseal /sim_post_vals'. iSmash.
     Qed.
-    Lemma csimv_constr_valₜ2 Φ tag eₛ eₜ :
+    Lemma rsimv_constr_valₜ2 Φ tag eₛ eₜ :
       SIM eₛ ⩾ eₜ [[ Χ ]] {{# (≈) }} -∗
       ( ∀ vₛ lₜ vₜ,
         (lₜ +ₗ 0) ↦ₜ tag -∗
@@ -338,11 +338,11 @@ Section sim_GS.
       SIM eₛ ⩾ &tag #() eₜ [[ Χ ]] {{# Φ }}.
     Proof.
       iIntros "Hsim HΦ".
-      iApply (csim_constr_valₜ2 with "Hsim").
+      iApply (rsim_constr_valₜ2 with "Hsim").
       rewrite sim_post_vals_unseal /sim_post_vals'. iSmash.
     Qed.
 
-    Lemma csimv_load Φ eₛ1 eₛ2 eₜ1 eₜ2 :
+    Lemma rsimv_load Φ eₛ1 eₛ2 eₜ1 eₜ2 :
       SIM eₛ1 ⩾ eₜ1 [[ Χ ]] {{# (≈) }} -∗
       SIM eₛ2 ⩾ eₜ2 [[ Χ ]] {{# (≈) }} -∗
       ( ∀ vₛ vₜ,
@@ -352,11 +352,11 @@ Section sim_GS.
       SIM ![eₛ2] eₛ1 ⩾ ![eₜ2] eₜ1 [[ Χ ]] {{# Φ }}.
     Proof.
       iIntros "Hsim1 Hsim2 HΦ".
-      iApply (csim_load with "Hsim1 Hsim2").
+      iApply (rsim_load with "Hsim1 Hsim2").
       rewrite sim_post_vals_unseal /sim_post_vals'. iSmash.
     Qed.
 
-    Lemma csimv_store Φ eₛ1 eₛ2 eₛ3 eₜ1 eₜ2 eₜ3 :
+    Lemma rsimv_store Φ eₛ1 eₛ2 eₛ3 eₜ1 eₜ2 eₜ3 :
       SIM eₛ1 ⩾ eₜ1 [[ Χ ]] {{# (≈) }} -∗
       SIM eₛ2 ⩾ eₜ2 [[ Χ ]] {{# (≈) }} -∗
       SIM eₛ3 ⩾ eₜ3 [[ Χ ]] {{# (≈) }} -∗
@@ -364,8 +364,8 @@ Section sim_GS.
       SIM eₛ1 <-[eₛ2]- eₛ3 ⩾ eₜ1 <-[eₜ2]- eₜ3 [[ Χ ]] {{# Φ }}.
     Proof.
       iIntros "Hsim1 Hsim2 Hsim3 HΦ".
-      iApply (csim_store with "Hsim1 Hsim2 Hsim3").
+      iApply (rsim_store with "Hsim1 Hsim2 Hsim3").
       rewrite sim_post_vals_unseal /sim_post_vals'. iSmash.
     Qed.
-  End csimv.
+  End rsimv.
 End sim_GS.
